Use RTS

games/Composition.v
@@ -4,244 +4,427 @@ Require Import Classical.
 Require Import Events.
 Require Import Smallstep.
 Require Import Behaviors.
-Require Import LTS.
+Require Import RTS.
 Require Import Trees.
 Require Import GameSemantics.
 Require Import ModuleSemantics.
 Require Import Classical.
+Require Import Axioms.
 
 
-(** * Resolution operator *)
+(** * Horizontal composition *)
 
-Module Res.
+Module HComp.
+  Import RTS.
 
-  (** ** Core transition system *)
+  Section RTS.
+    Context {G A} (sw : output G -> option (input G)) (α : rts G A).
 
-  Section RESOLVE.
-    Context {li : language_interface}.
-    Context (dom : query li -> bool).
-    Context {A} (α : lts (option (move (li -o li))) A) (a0 : A).
+    Inductive hc_state : Type :=
+      | hc_r (a : A) (k : input G -> A)
+      | hc_z.
 
-    Definition state : Type := list A.
-
-    Definition fcall q := Some (@qm (li -o li) (inr q)).
-    Definition fret  r := Some (@rm (li -o li) (inr r)).
-    Definition xcall q := Some (@rm (li -o li) (inl q)).
-    Definition xret  r := Some (@qm (li -o li) (inl r)).
-
-    Definition observable (at_outer_layer : Prop) (m : option (move (li -o li))) :=
-      match m with
-        | Some (rm (inr r)) => at_outer_layer
-        | Some (rm (inl q)) => dom q = false
-        | _ => True
+    Definition hc_behavior (r : RTS.behavior G A) (k : input G -> A) :=
+      match r with
+        | internal a =>
+          internal (hc_r a k)
+        | interacts mo k' =>
+          match sw mo with
+            | Some m => internal (hc_r (k m) k')
+            | None => interacts mo (fun mi => hc_r (k' mi) k)
+          end
+        | diverges =>
+          diverges
+        | goes_wrong =>
+          goes_wrong
       end.
 
-    Inductive step : option (move (li -o li)) -> relation state :=
-      | step_observable m a a' ks:
-          observable (ks = nil) m ->
-          α m a a' ->
-          step m (a :: ks) (a' :: ks)
-      | step_push q a k aq ks :
-          dom q = true ->
-          α (xcall q) a k ->
-          α (fcall q) a0 aq ->
-          step None (a :: ks) (aq :: k :: ks)
-      | step_pop r a a' k ar ks :
-          α (fret r) a a' ->
-          α (xret r) k ar ->
-          step None (a :: k :: ks) (ar :: ks).
+    Inductive hc : rts G hc_state :=
+      | hc_intro a k r :
+          α a r ->
+          hc (hc_r a k) (hc_behavior r k).
 
-  End RESOLVE.
+  End RTS.
 
-  (** ** Core commutation theorem *)
+  Arguments hc_state : clear implicits.
 
-  Section COMMUT.
-    Context {li} (L : semantics (li -o li)) (dom : query li -> bool).
+  (** ** Monotonicity *)
 
-    Inductive res_commut_st ks : rel _ (option (ModuleSemantics.Res.state L)) :=
-      | res_commut_st_none:
-          res_commut_st ks None None
-      | res_commut_st_some s:
-          res_commut_st ks s (Some (s, ks)).
+  Inductive hc_rel {G A B} R : rel (hc_state G A) (hc_state G B) :=
+    | hc_r_rel :
+        Monotonic hc_r (R ++> (- ==> R) ++> hc_rel R)
+    | hc_z_rel :
+        Monotonic hc_z (hc_rel R).
 
-    Hint Constructors res_commut_st.
+  Global Existing Instance hc_r_rel.
+  Global Existing Instance hc_z_rel.
+  Global Instance hc_r_rel_params : Params (@hc_r) 2.
 
-    Inductive res_commut_sim : rel _ _ :=
-      | res_commut_sim_waiting k ks :
-          res_commut_sim
-            (Behavior.waiting L k :: map (Behavior.waiting L) ks)
-            (Behavior.waiting (Res.semantics L dom) (Res.liftk L k ks))
-      | res_commut_sim_running_some t s rs ks :
-          res_commut_st ks s rs ->
-          res_commut_sim
-            (Behavior.running L t s :: map (Behavior.waiting L) ks)
-            (Behavior.running (Res.semantics L dom) t rs)
-      | res_commut_sim_wrong ks :
-          res_commut_sim
-            (Behavior.wrong L :: ks)
-            (Behavior.wrong (Res.semantics L dom)).
+  Global Instance hc_behavior_rel {G A B} R sw :
+    Monotonic
+      (hc_behavior sw)
+      (behavior_le R ++> (- ==> R) ++> behavior_le (@hc_rel G A B R)).
+  Proof.
+    unfold hc_behavior. rauto.
+  Qed.
 
-    Lemma commut_observable r ks :
-      ModuleSemantics.Res.observable L dom r ks <->
-      Res.observable dom (map (Behavior.waiting L) ks = nil) (Some (rm r)).
-    Proof.
-      simpl. unfold ModuleSemantics.Res.observable.
-      destruct r.
-      - reflexivity.
-      - split.
-        + intro. subst. reflexivity.
-        + destruct ks; simpl; congruence.
-    Qed.
+  Global Instance hc_behavior_rel_params :
+    Params (@hc_behavior) 2.
 
-    Lemma apply_cont_exists k q:
-      exists s, apply_cont L k q s.
-    Proof.
-      destruct (classic (exists s, k q s)) as [[s Hs] | Hns].
-      - exists (Some s). constructor. eauto.
-      - exists None. constructor. eauto.
-    Qed.
+  Global Instance hc_sim {G A B} R :
+    Monotonic hc (- ==> sim R ++> sim (@hc_rel G A B R)).
+  Proof.
+    intros sw α β Hαβ sa sb Hs ka Hka.
+    destruct Hka as [a ka ra].
+    inversion Hs as [xa b Hab xka kb Hk | ]; clear Hs; subst.
+    edestruct Hαβ as (rb & Hrb & Hr); eauto.
+    exists (hc_behavior sw rb kb). split; [ | rauto].
+    constructor; auto.
+  Qed.
 
-    Lemma commut_goes_wrong s ks:
-      (Nostep L s /\ forall r k, ~ final_state L s r k) <->
-      (Nostep (Res.semantics L dom) (Some s, ks) /\
-       forall r k, ~ final_state (Res.semantics L dom) (Some s, ks) r k).
-    Proof.
-      split.
-      - intros [Hns Hnf]. split.
-        + intros t s' Hs'.
-          inversion Hs'; clear Hs'; subst.
-          * eapply Hns; eauto.
-          * eapply Hnf; eauto.
-          * eapply Hnf; eauto.
-        + intros r k Hs.
-          inversion Hs; clear Hs; subst.
-          eapply Hnf; eauto.
-      - intros [Hns Hnf]. split.
-        + intros t s' Hs'.
-          eapply Hns. constructor. eauto.
-        + intros r k Hs.
-          destruct r as [q | r].
-          * destruct (dom q) eqn:Hq.
-            -- edestruct apply_cont_exists as [s' Hs'].
-               eapply Hns. eapply Res.step_call; eauto.
-            -- eapply Hnf. constructor; eauto.
-               simpl. assumption.
-          * destruct ks.
-            -- eapply Hnf. constructor; eauto.
-               simpl. reflexivity.
-            -- edestruct apply_cont_exists as [s' Hs'].
-               eapply Hns. eapply Res.step_return; eauto.
-    Qed.
+  Global Instance hc_sim_params :
+    Params (@hc) 2.
 
-    Lemma apply_cont_commut k q s ks:
-      let os := option_map (fun s => (Some s, ks)) s in
-      apply_cont L k q s ->
-      apply_cont (Res.semantics L dom) (Res.liftk L k ks) q os.
-    Proof.
-      intro; subst os.
-      destruct 1.
-      - constructor. constructor. assumption.
-      - constructor. intros s Hs. destruct Hs. eapply H; eauto.
-    Qed.
+  (** ** Properties *)
 
-    Lemma res_commut :
-      LTS.bisim res_commut_sim
-        (step dom (Behavior.step L) (Behavior.waiting L (initial_state L)))
-        (Behavior.step (Res.semantics L dom)).
-    Proof.
-      intros m s1 s2 Hs.
-      split.
-      - (* Forward *)
-        intros s1' Hs1'.
-        destruct Hs1'.
-        + (* observable step *)
-          destruct H0; inversion Hs; clear Hs; subst; simpl in H.
-          * eexists; split; constructor.
-            -- eapply apply_cont_commut; eauto.
-            -- destruct s; simpl; eauto.
-          * inversion H5; clear H5; subst.
-            eexists; split; constructor; constructor; eauto.
-          * eexists; split; constructor; eauto.
-          * inversion H5; clear H5; subst.
-            eexists; split; constructor; eauto.
-            constructor; eauto. apply commut_observable. simpl. auto.
-          * inversion H6; clear H6; subst.
-            eexists; split; constructor; eauto;
-            eapply commut_goes_wrong; eauto.
-          * inversion H4; clear H4; subst;
-            eexists; split; constructor; eauto.
-            -- intros t s' Hs'. inversion Hs'.
-            -- intros r k Hs. inversion Hs.
-        + (* push *)
-          inversion H0; clear H0; subst.
-          inversion Hs; clear Hs; subst.
-          inversion H6; clear H6; subst.
-          inversion H1; clear H1; subst.
-          change (?f ?hd :: map ?f ?tl) with (map f (hd :: tl)).
-          eexists. split.
-          * constructor. eapply Res.step_call; eauto.
-          * econstructor. destruct H4; constructor.
-        + (* pop *)
-          inversion H; clear H; subst.
-          inversion H0; clear H0; subst.
-          inversion Hs; clear Hs; subst.
-          inversion H5; clear H5; subst.
-          destruct ks0 as [ | xk xks]; try discriminate.
-          inversion H4; clear H4; subst.
-          eexists. split.
-          * constructor. eapply Res.step_return; eauto.
-          * constructor. destruct H1; constructor.
-      - (* Backward *)
-        intros s2' Hs2'.
-        destruct Hs2'; inversion Hs; clear Hs; subst.
-        + (* waiting -> running *)
-          destruct H.
-          * destruct H.
-            eexists; split; econstructor; simpl; eauto.
-            constructor. constructor; eauto.
-          * eexists; split; econstructor; simpl; eauto.
-            constructor. constructor; eauto.
-            intros s Hs. eapply H. constructor; eauto.
-        + (* running *)
-          inversion H2; clear H2; subst.
-          inversion H; clear H; subst.
-          * (* internal step *)
-            eexists; split; constructor; simpl; eauto.
-            constructor; eauto.
-          * (* call *)
-            eexists; split; [ | constructor; eauto]. simpl. econstructor.
-            -- eassumption.
-            -- constructor; eauto.
-            -- constructor; eauto.
-          * (* return *)
-            eexists. split.
-            -- eapply step_pop.
-               ++ constructor; eauto.
-               ++ constructor; eauto.
-            -- constructor; eauto.
-        + (* dequeue *)
-          eexists; split; constructor; simpl; eauto.
-          constructor.
-        + (* terminate *)
-          destruct H.
-          inversion H2; clear H2; subst.
-          apply commut_observable in H.
-          eexists; split; constructor; simpl; eauto.
-          constructor; eauto.
-        + (* go wrong *)
-          inversion H3; clear H3; subst.
-          destruct s0.
-          * edestruct (proj2 (commut_goes_wrong s ks)) as [Hns Hnf]; eauto.
-            eexists. split; constructor.
-            -- simpl. auto.
-            -- constructor; eauto.
-          * eexists. split; constructor.
-            -- simpl. auto.
-            -- constructor; eauto.
-        + inversion H1; clear H1; subst.
-          eexists; split; constructor; simpl; auto.
-          constructor.
-    Qed.
+  Lemma hc_behavior_external {G A} sw (r : behavior G A) (k : input G -> A) :
+    behavior_external (hc_behavior sw r k) ->
+    behavior_external r.
+  Proof.
+    destruct r; inversion 1; constructor.
+  Qed.
 
-  End COMMUT.
-End Res.
+  Lemma hc_reachable {G A} sw (α : rts G A) a a' k :
+    reachable α a a' ->
+    reachable (hc sw α) (hc_r a k) (hc_r a' k).
+  Proof.
+    induction 1; eauto.
+    econstructor; eauto.
+    change (internal _) with (hc_behavior sw (internal a') k).
+    constructor; eauto.
+  Qed.
+
+  (** ** Modules *)
+
+  Section HCOMP.
+    Context {li} (α1 α2 : modsem (li -o li)).
+
+    Definition hcomp_dom (q : query (li -o li)) : bool :=
+      modsem_dom α1 q || modsem_dom α2 q.
+
+    Definition hcomp_sw (q : reply (li -o li)) : option (query (li -o li)) :=
+      match q with
+        | inl q => if hcomp_dom (inr q) then Some (inr q) else None
+        | inr r => Some (inl r) (* XXX need to know whether outermost reply *)
+      end.
+
+    Definition hcomp_entry (q : query (li -o li)) :=
+      match modsem_dom α1 q, modsem_dom α2 q with
+        | true, false =>
+            hc_r (G := li -o li)
+              (inl (modsem_entry α1 q))
+              (fun m => inr (modsem_entry α2 m))
+        | false, true =>
+            hc_r (G := li -o li)
+              (inr (modsem_entry α2 q))
+              (fun m => inl (modsem_entry α1 m))
+        | _, _ =>
+            hc_z
+      end.
+
+    Definition hcomp : modsem (li -o li) :=
+      {|
+        modsem_lts := hc (G := li -o li) hcomp_sw (α1 + α2)%rts;
+        modsem_dom := hcomp_dom;
+        modsem_entry := hcomp_entry;
+      |}.
+  End HCOMP.
+
+  Global Instance hcomp_dom_ref :
+    Monotonic (@hcomp_dom) (forallr -, modref ++> modref ++> - ==> eq).
+  Proof.
+    unfold hcomp_dom. repeat rstep. f_equal; rauto.
+  Qed.
+
+  Global Instance hcomp_sw_ref :
+    Monotonic (@hcomp_sw) (forallr -, modref ++> modref ++> - ==> eq).
+  Proof.
+    unfold hcomp_sw. rauto.
+  Qed.
+
+  Global Instance hcomp_ref :
+    Monotonic (@hcomp) (forallr -, modref ++> modref ++> modref).
+  Proof.
+    intros li α1 β1 Hαβ1 α2 β2 Hαβ2.
+    pose proof Hαβ1 as [Hd1 R1 H1 He1].
+    pose proof Hαβ2 as [Hd2 R2 H2 He2].
+    exists (hc_rel (R1 + R2)); simpl.
+    - intros q. rauto.
+    - replace (hcomp_sw β1 β2) with (hcomp_sw α1 α2).
+      + eapply hc_sim. rauto.
+      + apply functional_extensionality. intros i. rauto.
+    - intros q. unfold hcomp_entry.
+      rewrite <- Hd1, <- Hd2.
+      repeat rstep; simpl; eauto.
+  Qed.
+
+  (** ** [hcomp] and [obs] *)
+
+  (** We prove that [hcomp] semi-commutes with [obs], in the sense
+    that applying [obs] after horizontal composition only should yield
+    the same result as applying it both before and after horizontal
+    composition. *)
+
+  CoInductive forever_switching {G A} sw (α : rts G A) : hc_state G A -> Prop :=
+    | forever_switching_intro a a' ra k s' :
+        reachable α a a' ->
+        α a' ra ->
+        behavior_external ra ->
+        hc_behavior sw ra k = internal s' ->
+        forever_switching sw α s' ->
+        forever_switching sw α (hc_r a k).
+
+  Lemma forever_switching_internal {G A} sw (α : rts G A) s s' :
+    hc sw α s (internal s') ->
+    forever_switching sw α s' ->
+    forever_switching sw α s.
+  Proof.
+    intros Hs' Hd.
+    inversion Hs' as [a0 k0 ra0 Hra0]; clear Hs'.
+    destruct ra0; inversion H0; clear H0.
+    - destruct Hd.
+      inversion H2; clear H2; subst.
+      eapply (forever_switching_intro sw α a0 a'0); eauto.
+    - destruct sw as [mx|] eqn:Hmx; inversion H2; clear H2; subst.
+      eapply (forever_switching_intro sw α a0 a0); eauto.
+      simpl. rewrite Hmx. reflexivity.
+  Qed.
+
+  Inductive hc_settles {G A} sw (α : rts G A) : rts G (hc_state G A) :=
+    | hc_settles_external a a' ra k r :
+        α a' ra ->
+        reachable α a a' ->
+        hc_behavior sw ra k = r ->
+        behavior_external r ->
+        hc_settles sw α (hc_r a k) r
+    | hc_settles_diverges a k :
+        forever_internal α a ->
+        hc_settles sw α (hc_r a k) diverges
+    | hc_settles_switch a a' ra k s' r :
+        α a' ra ->
+        reachable α a a' ->
+        behavior_external ra ->
+        hc_behavior sw ra k = internal s' ->
+        hc_settles sw α s' r ->
+        hc_settles sw α (hc_r a k) r.
+
+  Hint Constructors hc_settles.
+
+  Lemma hc_settles_internal {G A} sw (α : rts G A) s s' r :
+    hc sw α s (internal s') ->
+    hc_settles sw α s' r ->
+    hc_settles sw α s r.
+  Proof.
+    intros Hs' Hr.
+    inversion Hs' as [a k ra Hra]; clear Hs'; subst.
+    destruct ra; inversion H0; clear H0.
+    - destruct Hr; inversion H1; clear H1; subst.
+      + eapply (hc_settles_external sw α a a'0); eauto.
+      + eapply (hc_settles_diverges sw α a); eauto.
+        econstructor; eauto.
+      + eapply (hc_settles_switch sw α a a'0); eauto.
+    - destruct sw as [mx|] eqn:Hmx; inversion H1; clear H1; subst.
+      eapply (hc_settles_switch sw α a a (interacts m k0)); eauto.
+      simpl. rewrite Hmx. reflexivity.
+  Qed.
+
+  Inductive obs_hc {G A} sw (α : rts G A) : rts G (hc_state G A) :=
+    | obs_hc_settles s r :
+        hc_settles sw α s r ->
+        obs_hc sw α s r
+    | obs_hc_forever_switching s :
+        forever_switching sw α s ->
+        obs_hc sw α s diverges.
+
+  (** *** Alternative formulations for coinductive properties *)
+
+  Lemma forever_internal_nbr {G A} (α : rts G A) a :
+    nonbranching α ->
+    forever_internal α a <->
+    (forall a', reachable α a a' -> exists a'', α a' (internal a'')).
+  Proof.
+    intros Hα. split.
+    - intros Ha a' Ha'.
+      induction Ha' as [a | a a' a'' Ha' Ha'' IHa''].
+      + destruct Ha. eauto.
+      + eapply fi_inv_internal in Ha; eauto.
+    - revert a. cofix IH. intros a H.
+      destruct (H a) as (a' & Ha'); [ eauto .. | ].
+      econstructor; eauto.
+  Qed.
+
+  Lemma forever_switching_inv_internal {G A} sw (α : rts G A) s s' :
+    deterministic α ->
+    forever_switching sw α s ->
+    hc sw α s (internal s') ->
+    forever_switching sw α s'.
+  Proof.
+    intros Hα Hs Hs'.
+    inversion Hs'; clear Hs'; subst.
+    destruct r; simpl in H; try now inversion H.
+    - inversion Hs as [a1 a2 ra l s2 Ha2 Hra Hs2 Hs2d]; clear Hs; subst.
+      inversion H; clear H; subst.
+      eapply (reachable_inv_reachable α a a' a2) in Ha2; eauto.
+      econstructor; eauto.
+    - destruct sw eqn:Hm; inversion H; clear H; subst.
+      inversion Hs; clear Hs; subst.
+      assert (a' = a).
+      {
+        destruct H2; eauto.
+        eelim (nonbranching_internal_external α a (interacts m k0)); eauto.
+      }
+      subst.
+      assert (ra = interacts m k0).
+      {
+        eapply Hα; eauto.
+      }
+      subst.
+      simpl in H5.
+      rewrite Hm in H5.
+      inversion H5.
+      congruence.
+  Qed.
+
+  Lemma forever_switching_nbr {G A} sw (α : rts G A) s :
+    deterministic α ->
+    forever_switching sw α s <->
+    (s <> hc_z /\
+     forall a k, reachable (hc sw α) s (hc_r a k) ->
+                 exists a' r s', reachable α a a' /\
+                                 α a' r /\
+                                 behavior_external r /\
+                                 hc_behavior sw r k = internal s').
+  Proof.
+    intros Hα. split.
+    - intros Hs.
+      split. { destruct Hs. congruence. }
+      intros a k Hak.
+      remember (hc_r a k) as s' eqn:Hs' in Hak.
+      revert a k Hs'.
+      induction Hak; intros.
+      + destruct Hs.
+        inversion Hs'; clear Hs'; subst.
+        exists a', ra, s'. eauto.
+      + eapply IHHak; eauto.
+        eapply forever_switching_inv_internal; eauto.
+    - revert s. cofix IH. intros s [Hnz Hs].
+      destruct s as [a k | ]; try congruence.
+      edestruct (Hs a k) as (a' & r & s' & Ha' & Hr & Hrext & Hs'); [ eauto .. | ].
+      eapply (forever_switching_intro sw α a a' r k); eauto.
+      eapply IH.
+      split. { destruct r; simpl in Hs'; try congruence.
+               destruct sw; congruence. }
+      intros.
+      eapply Hs.
+      transitivity s'; auto.
+      transitivity (hc_r a' k); auto using hc_reachable.
+      econstructor; eauto.
+      rewrite <- Hs'. constructor. auto.
+  Qed.
+
+  Lemma hc_det {G A} sw (α : rts G A) :
+    deterministic α ->
+    deterministic (hc sw α).
+  Proof.
+    intros Hα s x y Hx Hy.
+    destruct Hx. inversion Hy.
+    f_equal; eauto.
+  Qed.
+
+  Lemma forever_hc {G A} sw (α : rts G A) s :
+    deterministic α ->
+    forever_internal (hc sw α) s ->
+    (exists a k, reachable (hc sw α) s (hc_r a k) /\ forever_internal α a) \/
+    forever_switching sw α s.
+  Proof.
+    intros Hα Hs1.
+    destruct (classic (forever_switching sw α s)) as [? | Hs2]; auto. left.
+    rewrite forever_internal_nbr in Hs1; eauto using hc_det.
+    rewrite forever_switching_nbr in Hs2; eauto.
+    apply not_and_or in Hs2 as [? | Hs2].
+    {
+      specialize (Hs1 s (reachable_refl _ s)) as (s' & Hs').
+      destruct Hs'. elim H. congruence.
+    }
+    apply not_all_ex_not in Hs2 as [a Hs2].
+    apply not_all_ex_not in Hs2 as [k Hs2].
+    apply not_all_ex_not in Hs2 as [Hak Hs2].
+    exists a, k. split; auto.
+    revert a Hak Hs2. cofix IH. intros.
+    edestruct (Hs1 _ Hak) as (a'' & Ha'').
+    inversion Ha''; clear Ha''; subst.
+    destruct r; try now inversion H2.
+    - simpl in H2. inversion H2; clear H2; subst.
+      econstructor; eauto.
+      eapply IH.
+      + transitivity (hc_r a k); eauto.
+        econstructor; eauto.
+        change (internal _) with (hc_behavior sw (internal a') k).
+        constructor; eauto.
+      + intros (a'' & r & s' & Ha'' & Hr & Hrext & Hs'); eauto 10.
+    - elim Hs2; eauto 10.
+  Qed.
+
+  Lemma obs_hc_obs_hc {G A} sw (α : rts G A) s r :
+    deterministic α ->
+    obs (hc sw α) s r ->
+    obs_hc sw α s r.
+  Proof.
+    intros Hα Hr.
+    destruct Hr as [Hs | s' r Hrext Hr Hs'].
+    - apply forever_hc in Hs as [(a & k & Hs' & Ha) | Hs]; auto.
+      + eapply obs_hc_settles.
+        remember (hc_r a k) as s' in Hs'.
+        induction Hs'; eauto using hc_settles_internal.
+        subst. constructor; auto.
+      + eapply obs_hc_forever_switching; eauto.
+    - eapply obs_hc_settles; eauto.
+      induction Hs'; eauto using hc_settles_internal.
+      inversion Hr; clear Hr; subst.
+      destruct r0; simpl in *; (try now inversion Hrext); eauto.
+  Qed.
+
+  Lemma obs_hc_obs_hc_obs {G A} sw (α : rts G A) s r :
+    obs_hc sw α s r ->
+    obs (hc sw (obs α)) s r.
+  Proof.
+    intro.
+    destruct H.
+    - induction H.
+      + apply obs_external with (hc_r a k); eauto.
+        subst. constructor.
+        eapply obs_external with a'; eauto.
+        eapply hc_behavior_external; eauto.
+      + apply obs_external with (hc_r a k); eauto.
+        change diverges with (hc_behavior sw diverges k).
+        constructor. auto.
+      + apply obs_reachable with s'; auto.
+        econstructor; eauto.
+        rewrite <- H2. constructor. eauto.
+    - eapply obs_diverges.
+      revert s H. cofix IH. intros.
+      destruct H. econstructor; eauto.
+      rewrite <- H2. constructor. eauto.
+  Qed.
+
+  Lemma obs_hc_obs_hc_obs_sim {G A} sw (α : rts G A) :
+    deterministic α ->
+    sim eq (obs (hc sw α)) (obs (hc sw (obs α))).
+  Proof.
+    intros Hα s _ [] r Hr.
+    exists r. split; [ | rauto].
+    apply obs_hc_obs_hc_obs.
+    apply obs_hc_obs_hc; auto.
+  Qed.
+
+End HComp.
